single_invocation_correctness.thy
@@ -2,6 +2,7 @@ section \<open>Single-Invocation Corrrectness\<close>
 
 theory single_invocation_correctness
   imports execution_invariants_s fixedpoints execution_invariants invContext_simps
+    state_monotonicGrowth_invariants
 begin
 
 
